\renewcommand{\O}{\mathcal{O}}
\newcommand{\tilo}{\widetilde{\O}}
\newcommand{\nil}{\varnothing}
\newcommand{\one}{\mathbbm{1}}
\newcommand{\bigO}{\mathcal{O}}
\DeclareMathOperator{\E}{\mathbb{E}}
\DeclareMathOperator{\Var}{\text{Var}}
\DeclareMathOperator{\Hom}{Hom}
\DeclareMathOperator{\rank}{rank}
\DeclareMathOperator{\sgn}{sgn}
\DeclareMathOperator{\Id}{Id}
\DeclareMathOperator{\img}{Img}
\DeclareMathOperator{\polylog}{\text{polylog}}
\DeclareMathOperator{\poly}{\text{poly}}
\newcommand{\st}{\text{ such that }}
\newcommand{\norm}[1]{\left\lVert#1\right\rVert}
\newcommand{\interior}[1]{ {\kern0pt#1}^{\mathrm{o}} }
\newcommand{\mb}{\mathbf}
\newcommand{\partition}{\vdash}
\newcommand{\x}{\mathbf{x}}
\newcommand{\y}{\mathbf{y}}
\newcommand{\z}{\mathbf{z}}
\newcommand{\eps}{\varepsilon}
\renewcommand{\d}{\mathrm{d}}
\renewcommand{\Re}{\mathrm{Re}}
\renewcommand{\Im}{\mathrm{Im}}
\newcommand{\legendre}[2]{\genfrac{(}{)}{}{}{#1}{#2}}
\newcommand{\EXP}{\mathsf{EXP}}
\newcommand{\PSPACE}{\mathsf{PSPACE}}
\newcommand{\NEXP}{\mathsf{NEXP}}
\newcommand{\PP}{\mathsf{P}}
\newcommand{\NP}{\mathsf{NP}}
\newcommand{\erdos}{Erd\H{o}s}
\newcommand{\pmo}{\set{-1,1}}
\newcommand{\zo}{\set{0,1}}


\newcommand{\setof}[2]{\left\{ #1\; : \;#2 \right\}}
\newcommand{\set}[1]{\left\{ #1\right\}}

\newcommand{\R}{\mathbb{R}}
\newcommand{\Q}{\mathbb{Q}}
\newcommand{\C}{\mathbb{C}}
\newcommand{\Z}{\mathbb{Z}}
\newcommand{\F}{\mathbb{F}}
\newcommand{\K}{\mathbb{K}}
\newcommand{\N}{\mathbb{N}}
\newcommand{\contr}{\[ \Rightarrow\!\Leftarrow \]}
\newcommand{\defeq}{\vcentcolon=}
\newcommand{\eqdef}{=\vcentcolon}

\newcommand{\floor}[1]{\left\lfloor #1 \right\rfloor}
\newcommand{\ceil}[1]{\left\lceil #1 \right\rceil}
\newcommand{\paren}[1]{\left( #1 \right)}
\newcommand{\ang}[1]{\langle #1 \rangle}
\newcommand{\abs}[1]{\left| #1 \right|}


Hilbert symbol:
$(a,b)=1$ if  $z^2-ax^2-by^2=0$ has a non-trivial solution and $-1$ else.

Norm map:
$N_{K/F}(\alpha)$ is the determinant of the map $x\mapsto \alpha
x$.
For example, 
If $K$ is an extension of $F$ by adjoining $\sqrt{\beta}$ then
$N(z+\sqrt{\beta}y) = z^2-\beta y^2.$

<div class="prop envbox">**Proposition.**
$(a,b)=1$ iff $a\in Nk[\sqrt{b}]^{*}$
</div>
<div class="pf envbox">**Proof.**
If $b$ is a square this is clear. 
If $b$ is a non-square then it is also true.
</div>

<div class="prop envbox">**Proposition.**
The hilbert symbol satisfies:
$(a,b)=(b,a)$,
$$(a,c^2)=(a,-a) = (a,1-a) = 1,$$
$$(a,b) =1 \implies (aa',b)=(a',b),$$
$$(a,b)=(a,-ab) = (a, (1-a)b).$$
</div>
<div class="pf envbox">**Proof.**
The implication $(a,b)=1\implies (aa',b)=(a',b)$ seems
interesting. 
It's true because we characterized  $\setof{x}{(x,b)=1}$ as $Nk[\sqrt{b}]^{*}$.
So, because $a\in Nk[\sqrt{b}]^{*}$ we have $aa'\in
Nk[\sqrt{b}]^{*} \iff a'\in Nk[\sqrt{b}]^{*}$.
</div>

<div class="lem envbox">**Lemma.**
$(aa',b)=(a,b)(a',b).$
</div>

Hilbert symbol is somehow related to legendre symbol.

# main theorem: some relationship between hilbert symbol and legendre symbol

<div class="thm envbox">**Theorem.**
In reals this is easy to compute. 
As always there is something different in the case that $p=2$.
We just state for odd $p$.

Write $a=p^{\alpha}u, b = p^{\beta}v.$
In the $p$-adics we have $(a,b) = (-1)^{\alpha \beta \eps(p)}
\legendre{u}{p}^{\beta} \legendre{v}{p}^{\alpha}$

where $\eps(u) =  \frac{u-1}{2}\mod 2$, 
and where legendre symbol of element of $\Z_p^{*}$ actually means
first take the element's reduction modulo $p$ and then take the
legendre symbol.
</div>

<div class="cor envbox">**Corollary.**
If $b$ is not a square then group $Nk_b^{*}$ is a subgroup of
index $2$ in $K^{*}$.
</div>

Recall: a point in $\Z_p^{m}$ is primitive if one of the $x_i$'s
in the vector is invertable (not div by $p$).

recall lemma: 
it you have non-trivial zero then you can find primitive zero.

now we have:
<div class="lem envbox">**Lemma.**
Let $v\in U$.
if $z^2-px^2-vy^2=0$ has nontrivial solution in $\Q_p$ then it
has one with $z,y\in U, x\in \Z_p$.
</div>
<div class="pf envbox">**Proof.**
First get a primitive zero. Then take stuff mod p it can't work
unless $z,y$ are units.

The proof is kind of interesting.
suppose our solution didn't have $y,z$ being units. Then at least one of
them is div by $p$. But taking reduction $\mod p$ we find that
both must be $0$. But then  $px^2\equiv  0 \mod p^2$ so $x,y,z$
all div by $p$ contradicting the primitiveness of the zero.
</div>

Now we prove the theorem

<div class="pf envbox">**Proof.**
Split to three cases.
The reason there are only three cases is by symmetry and the fact
that multiplying stuff by squares doesn't change the hilbert
symbol.

**Case 1:** $\alpha =\beta = 0$.
Then we want to prove $(u,v) = 1$.
The equation $z^2-ux^2-vy^2 = 0$ is a quadratic form in 3 vars so
has a solution modulo $p$. Furthermore, the discriminant of the
quadratic form  is a $p$-adic unit: $uv$. Thus by that other
lemma "newton's method" this lifts to a $p$-adic solution.

**Case 2:** $\alpha =0, \beta = 1$.
Here the claim is 
$$ (pu,v) = \legendre{v}{p} $$
Using a non-trivial fact from earlier in this blog post (the
first two propositions) we have in this case that $(pu,v)=(p,v)$.
If $v$ is a square then both $(p,v)$ and $\legendre{v}{p}$ are $1$ clearly.
Else, if $v$ is not a square then we had this theorem earlier
that said $p^{n}u$ is a square iff $n$ is even and $u\mod p$ is a
square in $\F_p$.
So then $\legendre{v}{p} = -1$.

Now using that lemma from earlier that somewhat conspicuously had
a $z^2-px^2-vy^2=0$ going on in it, an indication that it would
be useful for understanding $(v,p)$, we see that if  $(v,p)\neq
-1$ then we would get units $z,y$, and p-adic integer $x$ such that $z^2-px^2-vy^2=0$.
But this is ridiculous because then $v \equiv (zy^{-1})^2 \mod
p$, while we know $v$ is not a square.

**Case 3:** $\alpha =\beta = 1$.

We use another interesting formula, $(a,b)=(a,-ab)$ to reduce
this to case 2.

And the bilinearity thing follows from the fact that the legendre
symbols and other stuff in our formula is bilinear.

</div>

