{title}
overlap of simply periodic binary functions
{contents}

{description}
Let $f_a(x)$ denote a binary string consisting of  $a$ $0$'s
followed by $a$ $1$'s  and then repeating these $2a$ symbols.
We can equivalently describe $f_a$ as $f_a(x)= \floor{x/a}\bmod 2$.
We study $\sum_{x\in [ab]} f_a(x)\oplus f_b(x)$, in particular
bounding the difference of the sum from $\frac{ab}{2}$.
{body}

Let $f_a(x)$ denote a binary string consisting of  $a$ $0$'s
followed by $a$ $1$'s  and then repeating these $2a$ symbols.
We can equivalently describe $f_a$ as $f_a(x)= \floor{x/a}\bmod 2$.
We study $\sum_{x\in [ab]} f_a(x)\oplus f_b(x)$, in particular
bounding the difference of the sum from $\frac{ab}{2}$.

First, we reduce non-coprime $a,b$ to coprime $a,b$.
beg lem
  Fix $a,b\in \N$ with $d=\gcd(a,b)>1$.  Let $a_0=a/d,b_0=b/d.$
  Then $$\left|\sum_{x=1}^{ab} f_a(x)\oplus f_b(x)  - \frac{ab}{2}\right|\leq
  d^2\left|\sum_{x=1}^{a_0b_0}f_{a_0}(x)\oplus f_{b_0}(x) - \frac{a_0b_0}{2}\right|.$$
end lem
beg pf
We transform an $a_0 \times b_0$ grid and into a
$a\times b$ grid as follows: stretch each square into $d$
squares. Then duplicate the grid $d$ times, possibly inverting
the colors in even indexed duplicates.
This is a depiction of what is happening when we have $a,b$ not
coprime. This is why we can certainly bound the badness by $d^2$
times the badness before. And in general this is tight. That is,
for some $a,b$ it really will be $d^{2}$ times worse.
end pf

Now we analyze the main case: when $a,b$ are coprime.

beg lem
  Let $a,b$ be coprime. 
  Then $$\sum_{x=1}^{ab} f_a(x)\oplus f_b(x) = \ceil{ab/2}.$$
end lem
beg pf
  If $ab$ is even, there is a simple involution:
  $$x\mapsto ab-x.$$
  This involution is parity-xor flipping. This is great, this
  means that we get precisely $\frac{ab}{2}.$

  If $ab$ is odd, the situation is slightly more subtle. 
  Let $\lambda$ be the unique solution in $[ab]$ to the system
  $$\lambda \equiv 1 \bmod a, \;\; \lambda \equiv -1 \bmod b.$$
  The existence of $\lambda$ is guaranteed by the Chinese
  remainder theorem.
  Furthermore, if $\lambda = ka+1=c b -1$ then $k\equiv c \bmod
  2$ because $a,b$ are odd.
  Observe that $\lambda^2\equiv 1\bmod ab$. 
  This means that $x\mapsto \lambda x$ is an involution. 

  We separate the fixed points from the non-fixed points.
  $$\lambda x \equiv x \bmod ab \implies \lambda \equiv 0 \bmod
  b.$$

  To conclude the proof, we will show that:

- **Non-fixed points are sent to points with opposite
    parity-xor.**
- **Of the $a$ fixed points, $\ceil{a/2}$ have parity-xor of  $1$.**

**Claim 1**: Let $x$ be a non-fixed point, i.e., $x\not\equiv 0\bmod b$.
Then parity-xor of  $x,\lambda x$ are flipped.
This is because
$$\floor{ \lambda x / a} = \floor{(ka+1) / a} = k.$$
$$\floor{ \lambda x / b} = \floor{(cb-1) / b} = c-1.$$
But, we showed before $k\equiv c \mod 2$, so  $c-1\not\equiv k
\mod 2$.

**Claim 2**: Of the $a$ fixed points, $\ceil{a/2}$ have parity-xor of  $1$.

The map $yb \mapsto ab-yb$ is an involution of these points,
fixing only the middle point. Furthermore, for all
non-fixed-points, this involution flips the parity-xor.

To see this we do a simple computation:
$$\floor{yb / a}\oplus \floor{ yb / b} \equiv y \oplus \floor{yb
/ a}.$$
$$\floor{(ab-yb) / a}\oplus \floor{ (ab-yb) / b} \equiv a\oplus b \oplus y \oplus \floor{-yb
/ a}.$$
But of course $a\oplus b \equiv 0$ because  $a,b$ are both odd.
Finally, 
$$\floor{-yb / a}\not\equiv \floor{yb / a} \mod 2,$$
because their absolute values differ by exactly $1$.

This concludes the proof.
end pf

